src/Reflection/Z/Interpretations64/Relations.v
@@ -1,0 +1,531 @@
+Require Import Coq.ZArith.ZArith.
+Require Import Coq.micromega.Psatz.
+Require Import Crypto.Reflection.Z.Syntax.
+Require Import Crypto.Reflection.Syntax.
+Require Import Crypto.Reflection.Application.
+Require Import Crypto.Reflection.Z.InterpretationsGen.
+Require Import Crypto.Reflection.Z.Interpretations64.
+Require Import Crypto.ModularArithmetic.ModularBaseSystemListZOperationsProofs.
+Require Import Crypto.Util.Option.
+Require Import Crypto.Util.Bool.
+Require Import Crypto.Util.ZUtil.
+Require Import Crypto.Util.Prod.
+Require Import Crypto.Util.Tactics.
+
+Definition proj_eq_rel {A B} (proj : A -> B) (x : A) (y : B) : Prop
+  := proj x = y.
+Definition related'_Z {t} (x : BoundedWordW.BoundedWord) (y : Z.interp_base_type t) : Prop
+  := proj_eq_rel (BoundedWordW.to_Z' _) x y.
+Definition related_Z t : BoundedWordW.interp_base_type t -> Z.interp_base_type t -> Prop
+  := LiftOption.lift_relation (@related'_Z) t.
+Definition related'_wordW {t} (x : BoundedWordW.BoundedWord) (y : WordW.interp_base_type t) : Prop
+  := proj_eq_rel (BoundedWordW.to_wordW' _) x y.
+Definition related_wordW t : BoundedWordW.interp_base_type t -> WordW.interp_base_type t -> Prop
+  := LiftOption.lift_relation (@related'_wordW) t.
+Definition related_bounds t : BoundedWordW.interp_base_type t -> ZBounds.interp_base_type t -> Prop
+  := LiftOption.lift_relation2 (proj_eq_rel BoundedWordW.BoundedWordToBounds) t.
+
+Definition related_wordW_Z t : WordW.interp_base_type t -> Z.interp_base_type t -> Prop
+  := proj_eq_rel (WordW.to_Z _).
+
+Definition related'_wordW_bounds : WordW.wordW -> ZBounds.bounds -> Prop
+  := fun value b => (0 <= Bounds.lower b /\ Bounds.lower b <= WordW.wordWToZ value <= Bounds.upper b /\ Z.log2 (Bounds.upper b) < Z.of_nat WordW.bit_width)%Z.
+Definition related_wordW_bounds : WordW.wordW -> ZBounds.t -> Prop
+  := fun value b => match b with
+                    | Some b => related'_wordW_bounds value b
+                    | None => True
+                    end.
+Definition related_wordW_boundsi (t : base_type) : WordW.interp_base_type t -> ZBounds.interp_base_type t -> Prop
+  := match t with
+     | TZ => related_wordW_bounds
+     end.
+Definition related_wordW_boundsi' (t : base_type) : ZBounds.bounds -> WordW.interp_base_type t -> Prop
+  := match t return ZBounds.bounds -> WordW.interp_base_type t -> Prop with
+     | TZ => fun x y => related'_wordW_bounds y x
+     end.
+
+Local Notation related_op R interp_op1 interp_op2
+  := (forall (src dst : flat_type base_type) (op : op src dst)
+             (sv1 : interp_flat_type _ src) (sv2 : interp_flat_type _ src),
+         interp_flat_type_rel_pointwise2 R sv1 sv2 ->
+         interp_flat_type_rel_pointwise2 R (interp_op1 _ _ op sv1) (interp_op2 _ _ op sv2))
+       (only parsing).
+Local Notation related_const R interp f g
+  := (forall (t : base_type) (v : interp t), R t (f t v) (g t v))
+       (only parsing).
+
+Local Ltac related_const_t :=
+  let v := fresh in
+  let t := fresh in
+  intros t v; destruct t; intros; simpl in *; hnf; simpl;
+  cbv [BoundedWordW.wordWToBoundedWord related'_Z LiftOption.of' related_Z related_wordW related'_wordW proj_eq_rel] in *;
+  break_innermost_match; simpl;
+  first [ tauto
+        | Z.ltb_to_lt;
+          pose proof (WordW.wordWToZ_log_bound v);
+          try omega ].
+
+Lemma related_Z_const : related_const related_Z WordW.interp_base_type BoundedWordW.of_wordW WordW.to_Z.
+Proof. related_const_t. Qed.
+Lemma related_bounds_const : related_const related_bounds WordW.interp_base_type BoundedWordW.of_wordW ZBounds.of_wordW.
+Proof. related_const_t. Qed.
+Lemma related_wordW_const : related_const related_wordW WordW.interp_base_type BoundedWordW.of_wordW (fun _ x => x).
+Proof. related_const_t. Qed.
+
+Local Ltac related_wordW_op_t_step :=
+  first [ exact I
+        | reflexivity
+        | progress intros
+        | progress inversion_option
+        | progress ZBounds.inversion_bounds
+        | progress subst
+        | progress destruct_head' False
+        | progress destruct_head' prod
+        | progress destruct_head' and
+        | progress destruct_head' option
+        | progress destruct_head' BoundedWordW.BoundedWord
+        | progress cbv [related_wordW related_bounds related_Z LiftOption.lift_relation LiftOption.lift_relation2 LiftOption.of' smart_interp_flat_map BoundedWordW.BoundedWordToBounds BoundedWordW.to_bounds'] in *
+        | progress simpl @fst in *
+        | progress simpl @snd in *
+        | progress simpl @BoundedWord.upper in *
+        | progress simpl @BoundedWord.lower in *
+        | progress break_match
+        | progress break_match_hyps
+        | congruence
+        | match goal with
+          | [ H : ?op _ = Some _ |- _ ]
+            => let H' := fresh in
+               rename H into H';
+               first [ pose proof (@BoundedWordW.t_map1_correct _ _ _ _ _ H') as H; clear H'
+                     | pose proof (@BoundedWordW.t_map2_correct _ _ _ _ _ _ H') as H; clear H'
+                     | pose proof (@BoundedWordW.t_map4_correct _ _ _ _ _ _ H') as H; clear H' ];
+               simpl in H
+          | [ H : ?op _ = None |- _ ]
+            => let H' := fresh in
+               rename H into H';
+               first [ pose proof (@BoundedWordW.t_map1_correct_None _ _ _ _ H') as H; clear H'
+                     | pose proof (@BoundedWordW.t_map2_correct_None _ _ _ _ _ H') as H; clear H'
+                     | pose proof (@BoundedWordW.t_map4_correct_None _ _ _ _ _ H') as H; clear H' ];
+               simpl in H
+          end
+        | progress cbv [related'_wordW proj_eq_rel BoundedWordW.to_wordW' BoundedWordW.boundedWordToWordW BoundedWord.value] in *
+        | match goal with
+          | [ H : ?op None _ = Some _ |- _ ] => progress simpl in H
+          | [ H : ?op _ None = Some _ |- _ ] => progress simpl in H
+          | [ H : ?op (Some _) (Some _) = Some _ |- _ ] => progress simpl in H
+          | [ H : ?op (Some _) (Some _) = None |- _ ] => progress simpl in H
+          end ].
+Local Ltac related_wordW_op_t := repeat related_wordW_op_t_step.
+
+Lemma related_wordW_t_map1 opW opB pf
+      sv1 sv2
+  : interp_flat_type_rel_pointwise2 (t:=Tbase TZ) related_wordW sv1 sv2
+    -> @related_wordW TZ (BoundedWordW.t_map1 opW opB pf sv1) (opW sv2).
+Proof.
+  cbv [interp_flat_type BoundedWordW.interp_base_type ZBounds.interp_base_type LiftOption.interp_base_type' interp_flat_type_rel_pointwise2 interp_flat_type_rel_pointwise2_gen_Prop] in *.
+  related_wordW_op_t.
+Qed.
+
+Lemma related_wordW_t_map2 opW opB pf
+      sv1 sv2
+  : interp_flat_type_rel_pointwise2 (t:=Prod (Tbase TZ) (Tbase TZ)) related_wordW sv1 sv2
+    -> @related_wordW TZ (BoundedWordW.t_map2 opW opB pf (fst sv1) (snd sv1)) (opW (fst sv2) (snd sv2)).
+Proof.
+  cbv [interp_flat_type BoundedWordW.interp_base_type ZBounds.interp_base_type LiftOption.interp_base_type' interp_flat_type_rel_pointwise2 interp_flat_type_rel_pointwise2_gen_Prop] in *.
+  related_wordW_op_t.
+Qed.
+
+Lemma related_wordW_t_map4 opW opB pf
+      sv1 sv2
+  : interp_flat_type_rel_pointwise2 (t:=Prod (Prod (Prod (Tbase TZ) (Tbase TZ)) (Tbase TZ)) (Tbase TZ)) related_wordW sv1 sv2
+    -> @related_wordW TZ (BoundedWordW.t_map4 opW opB pf (fst (fst (fst sv1))) (snd (fst (fst sv1))) (snd (fst sv1)) (snd sv1))
+                       (opW (fst (fst (fst sv2))) (snd (fst (fst sv2))) (snd (fst sv2)) (snd sv2)).
+Proof.
+  cbv [interp_flat_type BoundedWordW.interp_base_type ZBounds.interp_base_type LiftOption.interp_base_type' interp_flat_type_rel_pointwise2 interp_flat_type_rel_pointwise2_gen_Prop] in *.
+  related_wordW_op_t.
+Qed.
+
+Lemma related_tuples_None_left
+      n T interp_base_type'
+      (R : forall t, LiftOption.interp_base_type' T t -> interp_base_type' t -> Prop)
+      (RNone : forall v, R TZ None v)
+      (v : interp_flat_type interp_base_type' (tuple (Tbase TZ) (S n)))
+  : interp_flat_type_rel_pointwise2
+      R
+      (flat_interp_untuple' (T:=Tbase TZ) (Tuple.push_option (n:=S n) None))
+      v.
+Proof.
+  induction n; simpl; intuition.
+Qed.
+
+Lemma related_tuples_Some_left
+      n T interp_base_type'
+      (R : forall t, T -> interp_base_type' t -> Prop)
+      u
+      (v : interp_flat_type interp_base_type' (tuple (Tbase TZ) (S n)))
+  : interp_flat_type_rel_pointwise2
+      R
+      (flat_interp_untuple' (T:=Tbase TZ) u)
+      v
+    <-> interp_flat_type_rel_pointwise2
+          (LiftOption.lift_relation R)
+          (flat_interp_untuple' (T:=Tbase TZ) (Tuple.push_option (n:=S n) (Some u)))
+          v.
+Proof.
+  induction n; [ reflexivity | ].
+  simpl in *; rewrite <- IHn; clear IHn.
+  reflexivity.
+Qed.
+
+Lemma related_tuples_Some_left_ext
+      {n T interp_base_type'}
+      {R : forall t, T -> interp_base_type' t -> Prop}
+      {u v u'}
+      (H : Tuple.lift_option (flat_interp_tuple (T:=Tbase TZ) (n:=S n) u) = Some u')
+  : interp_flat_type_rel_pointwise2
+      R
+      (flat_interp_untuple' (T:=Tbase TZ) u') v
+    <-> interp_flat_type_rel_pointwise2
+          (LiftOption.lift_relation R)
+          u v.
+Proof.
+  induction n.
+  { simpl in *; subst; reflexivity. }
+  { destruct_head_hnf' prod.
+    simpl in H; break_match_hyps; inversion_option; inversion_prod; subst.
+    simpl; rewrite <- IHn by eassumption; clear IHn.
+    reflexivity. }
+Qed.
+
+Lemma related_tuples_proj_eq_rel_untuple
+      {n T interp_base_type'}
+      {proj : forall t, T -> interp_base_type' t}
+      {u : Tuple.tuple _ (S n)} {v : Tuple.tuple _ (S n)}
+  : interp_flat_type_rel_pointwise2
+      (fun t => proj_eq_rel (proj t))
+      (flat_interp_untuple' (T:=Tbase TZ) u)
+      (flat_interp_untuple' (T:=Tbase TZ) v)
+    <-> (Tuple.map (proj _) u = v).
+Proof.
+  induction n; [ reflexivity | ].
+  destruct_head_hnf' prod.
+  simpl @Tuple.tuple.
+  rewrite !Tuple.map_S, path_prod_uncurried_iff, <- prod_iff_and; unfold fst, snd.
+  rewrite <- IHn.
+  reflexivity.
+Qed.
+
+Lemma related_tuples_proj_eq_rel_tuple
+      {n T interp_base_type'}
+      {proj : forall t, T -> interp_base_type' t}
+      {u v}
+  : interp_flat_type_rel_pointwise2
+      (fun t => proj_eq_rel (proj t))
+      u v
+    <-> (Tuple.map (proj _) (flat_interp_tuple (n:=S n) (T:=Tbase TZ) u)
+         = flat_interp_tuple (T:=Tbase TZ) v).
+Proof.
+  rewrite <- related_tuples_proj_eq_rel_untuple, !flat_interp_untuple'_tuple; reflexivity.
+Qed.
+
+Local Arguments LiftOption.lift_relation2 _ _ _ _ !_ !_ / .
+Lemma related_tuples_lift_relation2_untuple'
+      n T U
+      (R : T -> U -> Prop)
+      (t : option (Tuple.tuple T (S n)))
+      (u : option (Tuple.tuple U (S n)))
+  : interp_flat_type_rel_pointwise2
+      (LiftOption.lift_relation2 R)
+      (flat_interp_untuple' (T:=Tbase TZ) (Tuple.push_option t))
+      (flat_interp_untuple' (T:=Tbase TZ) (Tuple.push_option u))
+    <-> LiftOption.lift_relation2
+          (interp_flat_type_rel_pointwise2 (fun _ => R))
+          TZ
+          (option_map (flat_interp_untuple' (interp_base_type:=fun _ => T) (T:=Tbase TZ)) t)
+          (option_map (flat_interp_untuple' (interp_base_type:=fun _ => U) (T:=Tbase TZ)) u).
+Proof.
+  induction n.
+  { destruct_head' option; reflexivity. }
+  { specialize (IHn (option_map (@fst _ _) t) (option_map (@fst _ _) u)).
+    destruct_head' option;
+      destruct_head_hnf' prod;
+      simpl @option_map in *;
+      simpl @LiftOption.lift_relation2 in *;
+      try (rewrite <- IHn; reflexivity);
+      try (simpl @interp_flat_type_rel_pointwise2; tauto). }
+Qed.
+
+Lemma related_tuples_lift_relation2_untuple'_ext
+      {n T U}
+      {R : T -> U -> Prop}
+      {t u}
+      (H : (exists v, Tuple.lift_option (n:=S n) (flat_interp_tuple (T:=Tbase TZ) t) = Some v)
+           \/ (exists v, Tuple.lift_option (n:=S n) (flat_interp_tuple (T:=Tbase TZ) u) = Some v))
+  : interp_flat_type_rel_pointwise2
+      (LiftOption.lift_relation2 R)
+      t u
+    <-> LiftOption.lift_relation2
+          (interp_flat_type_rel_pointwise2 (fun _ => R))
+          TZ
+          (option_map (flat_interp_untuple' (interp_base_type:=fun _ => T) (T:=Tbase TZ)) (Tuple.lift_option (flat_interp_tuple (T:=Tbase TZ) t)))
+          (option_map (flat_interp_untuple' (interp_base_type:=fun _ => U) (T:=Tbase TZ)) (Tuple.lift_option (flat_interp_tuple (T:=Tbase TZ) u))).
+Proof.
+  induction n.
+  { destruct_head_hnf' option; reflexivity. }
+  { specialize (IHn (fst t) (fst u)).
+    lazymatch type of IHn with
+    | ?T -> _ => let H := fresh in assert (H : T); [ | specialize (IHn H); clear H ]
+    end.
+    { destruct_head' or; [ left | right ]; destruct_head' ex; destruct_head_hnf' prod; eexists;
+        (etransitivity;
+         [ | first [ refine (f_equal (option_map (@fst _ _)) (_ : _ = Some (_, _))); eassumption
+                   | refine (f_equal (option_map (@snd _ _)) (_ : _ = Some (_, _))); eassumption ] ]);
+        instantiate; simpl in *; break_match; simpl in *; congruence. }
+    destruct_head_hnf' prod;
+      destruct_head_hnf' option;
+      simpl @fst in *; simpl @snd in *;
+        (etransitivity; [ simpl @interp_flat_type_rel_pointwise2 | reflexivity ]);
+        try solve [ repeat first [ progress simpl in *
+                                 | tauto
+                                 | congruence
+                                 | progress destruct_head ex
+                                 | progress destruct_head or
+                                 | progress break_match ] ]. }
+Qed.
+
+Lemma lift_option_flat_interp_tuple'
+      {n T x y}
+  : (Tuple.lift_option (n:=S n) (A:=T) (flat_interp_tuple' (interp_base_type:=LiftOption.interp_base_type' _) (T:=Tbase TZ) x) = Some y)
+    <-> (x = flat_interp_untuple' (T:=Tbase TZ) (n:=n) (Tuple.push_option (n:=S n) (Some y))).
+Proof.
+  rewrite Tuple.push_lift_option; generalize (Tuple.push_option (Some y)); intro.
+  split; intro; subst;
+    rewrite ?flat_interp_tuple'_untuple', ?flat_interp_untuple'_tuple';
+    reflexivity.
+Qed.
+
+Lemma lift_option_None_interp_flat_type_rel_pointwise2_1
+      T U n R x y
+      (H : interp_flat_type_rel_pointwise2 (LiftOption.lift_relation2 R) x y)
+      (HNone : Tuple.lift_option (A:=T) (n:=S n) (flat_interp_tuple' (T:=Tbase TZ) (n:=n) x) = None)
+  : Tuple.lift_option (A:=U) (n:=S n) (flat_interp_tuple' (T:=Tbase TZ) (n:=n) y) = None.
+Proof.
+  induction n; [ | specialize (IHn (fst x) (fst y) (proj1 H)) ];
+    repeat first [ progress destruct_head_hnf' False
+                 | reflexivity
+                 | progress inversion_option
+                 | progress simpl in *
+                 | progress subst
+                 | progress specialize_by congruence
+                 | progress destruct_head_hnf' prod
+                 | progress destruct_head_hnf' and
+                 | progress destruct_head_hnf' option
+                 | progress break_match
+                 | progress break_match_hyps ].
+Qed.
+
+Local Arguments LiftOption.lift_relation _ _ _ _ !_ _ / .
+Local Arguments LiftOption.of' _ _ !_ / .
+Local Arguments BoundedWordW.BoundedWordToBounds !_ / .
+
+Lemma related_wordW_op : related_op related_wordW (@BoundedWordW.interp_op) (@WordW.interp_op).
+Proof.
+  (let op := fresh in intros ?? op; destruct op; simpl);
+    try first [ apply related_wordW_t_map1
+              | apply related_wordW_t_map2
+              | apply related_wordW_t_map4 ].
+Qed.
+
+Lemma related_bounds_t_map1 opW opB pf
+      (HN : opB None = None)
+      sv1 sv2
+  : interp_flat_type_rel_pointwise2 (t:=Tbase TZ) related_bounds sv1 sv2
+    -> @related_bounds TZ (BoundedWordW.t_map1 opW opB pf sv1) (opB sv2).
+Proof.
+  cbv [interp_flat_type BoundedWordW.interp_base_type ZBounds.interp_base_type LiftOption.interp_base_type' interp_flat_type_rel_pointwise2 interp_flat_type_rel_pointwise2_gen_Prop] in *.
+  related_wordW_op_t.
+Qed.
+
+Lemma related_bounds_t_map2 opW opB pf
+      (HN0 : forall v, opB None v = None)
+      (HN1 : forall v, opB v None = None)
+      sv1 sv2
+  : interp_flat_type_rel_pointwise2 (t:=Prod (Tbase TZ) (Tbase TZ)) related_bounds sv1 sv2
+    -> @related_bounds TZ (BoundedWordW.t_map2 opW opB pf (fst sv1) (snd sv1)) (opB (fst sv2) (snd sv2)).
+Proof.
+  cbv [interp_flat_type BoundedWordW.interp_base_type ZBounds.interp_base_type LiftOption.interp_base_type' interp_flat_type_rel_pointwise2 interp_flat_type_rel_pointwise2_gen_Prop] in *.
+  related_wordW_op_t.
+Qed.
+
+Lemma related_bounds_t_map4 opW opB pf
+      (HN0 : forall x y z, opB None x y z = None)
+      (HN1 : forall x y z, opB x None y z = None)
+      (HN2 : forall x y z, opB x y None z = None)
+      (HN3 : forall x y z, opB x y z None = None)
+      sv1 sv2
+  : interp_flat_type_rel_pointwise2 (t:=Prod (Prod (Prod (Tbase TZ) (Tbase TZ)) (Tbase TZ)) (Tbase TZ)) related_bounds sv1 sv2
+    -> @related_bounds TZ (BoundedWordW.t_map4 opW opB pf (fst (fst (fst sv1))) (snd (fst (fst sv1))) (snd (fst sv1)) (snd sv1))
+                       (opB (fst (fst (fst sv2))) (snd (fst (fst sv2))) (snd (fst sv2)) (snd sv2)).
+Proof.
+  cbv [interp_flat_type BoundedWordW.interp_base_type ZBounds.interp_base_type LiftOption.interp_base_type' interp_flat_type_rel_pointwise2 interp_flat_type_rel_pointwise2_gen_Prop] in *.
+  destruct_head prod.
+  intros; destruct_head' prod.
+  progress cbv [related_wordW related_bounds related_Z LiftOption.lift_relation LiftOption.lift_relation2 LiftOption.of' smart_interp_flat_map BoundedWordW.BoundedWordToBounds BoundedWordW.to_bounds' proj_eq_rel] in *.
+  destruct_head' option; destruct_head_hnf' and; destruct_head_hnf' False; subst;
+    try solve [ simpl; rewrite ?HN0, ?HN1, ?HN2, ?HN3; tauto ];
+    [].
+  related_wordW_op_t.
+Qed.
+
+Local Arguments Tuple.lift_option : simpl never.
+Local Arguments Tuple.push_option : simpl never.
+Local Arguments Tuple.map : simpl never.
+Local Arguments Tuple.map2 : simpl never.
+
+Local Arguments ZBounds.SmartBuildBounds _ _ / .
+Lemma related_bounds_op : related_op related_bounds (@BoundedWordW.interp_op) (@ZBounds.interp_op).
+Proof.
+  let op := fresh in intros ?? op; destruct op; simpl.
+  { apply related_bounds_t_map2; intros; destruct_head' option; reflexivity. }
+  { apply related_bounds_t_map2; intros; destruct_head' option; reflexivity. }
+  { apply related_bounds_t_map2; intros; destruct_head' option; reflexivity. }
+  { apply related_bounds_t_map2; intros; destruct_head' option; reflexivity. }
+  { apply related_bounds_t_map2; intros; destruct_head' option; reflexivity. }
+  { apply related_bounds_t_map2; intros; destruct_head' option; reflexivity. }
+  { apply related_bounds_t_map2; intros; destruct_head' option; reflexivity. }
+  { apply related_bounds_t_map1; intros; destruct_head' option; unfold ZBounds.neg; break_match; reflexivity. }
+  { apply related_bounds_t_map4; intros; destruct_head' option; reflexivity. }
+  { apply related_bounds_t_map4; intros; destruct_head' option; reflexivity. }
+Qed.
+
+Local Ltac WordW.Rewrites.wordW_util_arith ::=
+      solve [ autorewrite with Zshift_to_pow; omega
+            | autorewrite with Zshift_to_pow; nia
+            | autorewrite with Zshift_to_pow; auto with zarith
+            | eapply Z.le_lt_trans; [ eapply Z.log2_le_mono | eassumption ];
+              autorewrite with Zshift_to_pow; auto using Z.mul_le_mono_nonneg with zarith;
+              solve [ omega
+                    | nia
+                    | etransitivity; [ eapply Z.div_le_mono | eapply Z.div_le_compat_l ];
+                      auto with zarith ]
+            | apply Z.land_nonneg; WordW.Rewrites.wordW_util_arith
+            | eapply Z.le_lt_trans; [ eapply Z.log2_le_mono | eassumption ];
+              instantiate; apply Z.min_case_strong; intros;
+              first [ etransitivity; [ apply Z.land_upper_bound_l | ]; omega
+                    | etransitivity; [ apply Z.land_upper_bound_r | ]; omega ]
+            | rewrite Z.log2_lor by omega;
+              apply Z.max_case_strong; intro;
+              (eapply Z.le_lt_trans; [ eapply Z.log2_le_mono; eassumption | assumption ])
+            | eapply Z.le_lt_trans; [ eapply Z.log2_le_mono, neg_upperbound | ];
+              WordW.Rewrites.wordW_util_arith
+            | (progress unfold ModularBaseSystemListZOperations.cmovne, ModularBaseSystemListZOperations.cmovl, ModularBaseSystemListZOperations.neg); break_match;
+              WordW.Rewrites.wordW_util_arith ].
+Local Ltac related_Z_op_t_step :=
+  first [ progress related_wordW_op_t_step
+        | progress cbv [related'_Z proj_eq_rel BoundedWordW.to_Z' BoundedWordW.to_wordW' WordW.to_Z BoundedWordW.boundedWordToWordW BoundedWord.value] in *
+        | autorewrite with push_wordWToZ ].
+Local Ltac related_Z_op_t := repeat related_Z_op_t_step.
+
+Local Notation is_bounded_by value lower upper
+  := ((0 <= lower /\ lower <= WordW.wordWToZ value <= upper /\ Z.log2 upper < Z.of_nat WordW.bit_width)%Z)
+       (only parsing).
+Local Notation is_in_bounds value bounds
+  := (is_bounded_by value (Bounds.lower bounds) (Bounds.upper bounds))
+       (only parsing).
+
+Lemma related_Z_t_map1 opZ opW opB pf
+      (H : forall x bxs brs,
+          Some brs = opB (Some bxs)
+          -> is_in_bounds x bxs
+          -> is_in_bounds (opW x) brs
+          -> WordW.wordWToZ (opW x) = (opZ (WordW.wordWToZ x)))
+      sv1 sv2
+  : interp_flat_type_rel_pointwise2 (t:=Tbase TZ) related_Z sv1 sv2
+    -> @related_Z TZ (BoundedWordW.t_map1 opW opB pf sv1) (opZ sv2).
+Proof.
+  cbv [interp_flat_type BoundedWordW.interp_base_type ZBounds.interp_base_type LiftOption.interp_base_type' interp_flat_type_rel_pointwise2 interp_flat_type_rel_pointwise2_gen_Prop] in *.
+  related_Z_op_t.
+  eapply H; eauto.
+Qed.
+
+Lemma related_Z_t_map2 opZ opW opB pf
+      (H : forall x y bxs bys brs,
+          Some brs = opB (Some bxs) (Some bys)
+          -> is_in_bounds x bxs
+          -> is_in_bounds y bys
+          -> is_in_bounds (opW x y) brs
+          -> WordW.wordWToZ (opW x y) = (opZ (WordW.wordWToZ x) (WordW.wordWToZ y)))
+      sv1 sv2
+  : interp_flat_type_rel_pointwise2 (t:=Prod (Tbase TZ) (Tbase TZ)) related_Z sv1 sv2
+    -> @related_Z TZ (BoundedWordW.t_map2 opW opB pf (fst sv1) (snd sv1)) (opZ (fst sv2) (snd sv2)).
+Proof.
+  cbv [interp_flat_type BoundedWordW.interp_base_type ZBounds.interp_base_type LiftOption.interp_base_type' interp_flat_type_rel_pointwise2 interp_flat_type_rel_pointwise2_gen_Prop] in *.
+  related_Z_op_t.
+  eapply H; eauto.
+Qed.
+
+Lemma related_Z_t_map4 opZ opW opB pf
+      (H : forall x y z w bxs bys bzs bws brs,
+          Some brs = opB (Some bxs) (Some bys) (Some bzs) (Some bws)
+          -> is_in_bounds x bxs
+          -> is_in_bounds y bys
+          -> is_in_bounds z bzs
+          -> is_in_bounds w bws
+          -> is_in_bounds (opW x y z w) brs
+          -> WordW.wordWToZ (opW x y z w) = (opZ (WordW.wordWToZ x) (WordW.wordWToZ y) (WordW.wordWToZ z) (WordW.wordWToZ w)))
+      sv1 sv2
+  : interp_flat_type_rel_pointwise2 (t:=(Tbase TZ * Tbase TZ * Tbase TZ * Tbase TZ)%ctype) related_Z sv1 sv2
+    -> @related_Z TZ (BoundedWordW.t_map4 opW opB pf (fst (fst (fst sv1))) (snd (fst (fst sv1))) (snd (fst sv1)) (snd sv1))
+                  (opZ (fst (fst (fst sv2))) (snd (fst (fst sv2))) (snd (fst sv2)) (snd sv2)).
+Proof.
+  cbv [interp_flat_type BoundedWordW.interp_base_type ZBounds.interp_base_type LiftOption.interp_base_type' interp_flat_type_rel_pointwise2 interp_flat_type_rel_pointwise2_gen_Prop] in *.
+  related_Z_op_t.
+  eapply H; eauto.
+Qed.
+
+Local Arguments related_Z _ !_ _ / .
+
+Local Arguments related'_Z _ _ _ / .
+
+Local Ltac related_Z_op_fin_t_step :=
+  first [ progress subst
+        | progress inversion_option
+        | progress ZBounds.inversion_bounds
+        | progress destruct_head' Bounds.bounds
+        | progress destruct_head' ZBounds.bounds
+        | progress destruct_head' and
+        | progress simpl in * |-
+        | progress break_match_hyps
+        | congruence
+        | progress inversion_option
+        | intro
+        | progress autorewrite with push_wordWToZ
+        | match goal with
+          | [ H : andb _ _ = true |- _ ] => rewrite Bool.andb_true_iff in H
+          | [ H : context[Tuple.lift_option (Tuple.push_option _)] |- _ ]
+            => rewrite Tuple.lift_push_option in H
+          end
+        | progress Z.ltb_to_lt ].
+Local Ltac related_Z_op_fin_t := repeat related_Z_op_fin_t_step.
+
+Local Opaque WordW.bit_width.
+
+Local Arguments ZBounds.neg _ !_ / .
+
+Lemma related_Z_op : related_op related_Z (@BoundedWordW.interp_op) (@Z.interp_op).
+Proof.
+  let op := fresh in intros ?? op; destruct op; simpl.
+  { apply related_Z_t_map2; related_Z_op_fin_t. }
+  { apply related_Z_t_map2; related_Z_op_fin_t. }
+  { apply related_Z_t_map2; related_Z_op_fin_t. }
+  { apply related_Z_t_map2; related_Z_op_fin_t. }
+  { apply related_Z_t_map2; related_Z_op_fin_t. }
+  { apply related_Z_t_map2; related_Z_op_fin_t. }
+  { apply related_Z_t_map2; related_Z_op_fin_t. }
+  { apply related_Z_t_map1; related_Z_op_fin_t. }
+  { apply related_Z_t_map4; related_Z_op_fin_t. }
+  { apply related_Z_t_map4; related_Z_op_fin_t. }
+Qed.
+
+Create HintDb interp_related discriminated.
+Hint Resolve related_Z_op related_bounds_op related_wordW_op related_Z_const related_bounds_const related_wordW_const : interp_related.
