src/Reflection/Z/Interpretations64/RelationsCombinations.v
@@ -1,0 +1,359 @@
+Require Import Coq.ZArith.ZArith.
+Require Import Crypto.Reflection.Z.Syntax.
+Require Import Crypto.Reflection.Syntax.
+Require Import Crypto.Reflection.Application.
+Require Import Crypto.Reflection.Z.InterpretationsGen.
+Require Import Crypto.Reflection.Z.Interpretations64.
+Require Import Crypto.Reflection.Z.Interpretations64.Relations.
+Require Import Crypto.Util.Option.
+Require Import Crypto.Util.Bool.
+Require Import Crypto.Util.ZUtil.
+Require Import Crypto.Util.Prod.
+Require Import Crypto.Util.Tactics.
+
+Module Relations.
+  Section lift.
+    Context {interp_base_type1 interp_base_type2 : base_type -> Type}
+            (R : forall t, interp_base_type1 t -> interp_base_type2 t -> Prop).
+
+    Definition interp_type_rel_pointwise2_uncurried
+               {t : type base_type}
+      := match t return interp_type interp_base_type1 t -> interp_type interp_base_type2 t -> _ with
+         | Tflat T => fun f g => interp_flat_type_rel_pointwise2 (t:=T) R f g
+         | Arrow A B
+           => fun f g
+              => forall x y, interp_flat_type_rel_pointwise2 R x y
+                             -> interp_flat_type_rel_pointwise2 R (ApplyInterpedAll f x) (ApplyInterpedAll g y)
+         end.
+
+    Lemma uncurry_interp_type_rel_pointwise2
+          {t f g}
+      : interp_type_rel_pointwise2 (t:=t) R f g
+        <-> interp_type_rel_pointwise2_uncurried (t:=t) f g.
+    Proof.
+      unfold interp_type_rel_pointwise2_uncurried.
+      induction t as [|A B IHt]; [ reflexivity | ].
+      { simpl; unfold Morphisms.respectful_hetero in *; destruct B.
+        { reflexivity. }
+        { setoid_rewrite IHt; clear IHt.
+          split; intro H; intros.
+          { simpl in *; intuition. }
+          { eapply (H (_, _) (_, _)); simpl in *; intuition. } } }
+    Qed.
+  End lift.
+
+  Section proj.
+    Context {interp_base_type1 interp_base_type2}
+            (proj : forall t : base_type, interp_base_type1 t -> interp_base_type2 t).
+
+    Let R {t : flat_type base_type} f g :=
+      SmartVarfMap (t:=t) proj f = g.
+
+    Definition interp_type_rel_pointwise2_uncurried_proj
+               {t : type base_type}
+      : interp_type interp_base_type1 t -> interp_type interp_base_type2 t -> Prop
+      := match t return interp_type interp_base_type1 t -> interp_type interp_base_type2 t -> Prop  with
+         | Tflat T => @R _
+         | Arrow A B
+           => fun f g
+              => forall x : interp_flat_type interp_base_type1 (all_binders_for (Arrow A B)),
+                  let y := SmartVarfMap proj x in
+                  let fx := ApplyInterpedAll f x in
+                  let gy := ApplyInterpedAll g y in
+                  @R _ fx gy
+         end.
+
+    Lemma uncurry_interp_type_rel_pointwise2_proj
+          {t : type base_type}
+          {f : interp_type interp_base_type1 t}
+          {g}
+      : interp_type_rel_pointwise2 (t:=t) (fun t => @R _) f g
+        -> interp_type_rel_pointwise2_uncurried_proj (t:=t) f g.
+    Proof.
+      unfold interp_type_rel_pointwise2_uncurried_proj.
+      induction t as [t|A B IHt]; simpl; unfold Morphisms.respectful_hetero in *.
+      { induction t as [t|A IHA B IHB]; simpl; [ solve [ trivial | reflexivity ] | ].
+        intros [HA HB].
+        specialize (IHA _ _ HA); specialize (IHB _ _ HB).
+        unfold R in *.
+        repeat first [ progress destruct_head_hnf' prod
+                     | progress simpl in *
+                     | progress subst
+                     | reflexivity ]. }
+      { destruct B; intros H ?; apply IHt, H; clear IHt;
+          repeat first [ reflexivity
+                       | progress simpl in *
+                       | progress unfold R, LiftOption.of' in *
+                       | progress break_match ]. }
+    Qed.
+  End proj.
+
+  Section proj_option.
+    Context {interp_base_type1 : Type} {interp_base_type2 : base_type -> Type}
+            (proj_option : forall t, interp_base_type1 -> interp_base_type2 t).
+
+    Let R {t : flat_type base_type} f g :=
+      let f' := LiftOption.of' (t:=t) f in
+      match f' with
+      | Some f' => SmartVarfMap proj_option f' = g
+      | None => True
+      end.
+
+    Definition interp_type_rel_pointwise2_uncurried_proj_option
+               {t : type base_type}
+      : interp_type (LiftOption.interp_base_type' interp_base_type1) t -> interp_type interp_base_type2 t -> Prop
+      := match t return interp_type (LiftOption.interp_base_type' interp_base_type1) t -> interp_type interp_base_type2 t -> Prop  with
+         | Tflat T => @R _
+         | Arrow A B
+           => fun f g
+              => forall x : interp_flat_type (fun _ => interp_base_type1) (all_binders_for (Arrow A B)),
+                  let y := SmartVarfMap proj_option x in
+                  let fx := ApplyInterpedAll f (LiftOption.to' (Some x)) in
+                  let gy := ApplyInterpedAll g y in
+                  @R _ fx gy
+         end.
+
+    Lemma uncurry_interp_type_rel_pointwise2_proj_option
+          {t : type base_type}
+          {f : interp_type (LiftOption.interp_base_type' interp_base_type1) t}
+          {g}
+      : interp_type_rel_pointwise2 (t:=t) (fun t => @R _) f g
+        -> interp_type_rel_pointwise2_uncurried_proj_option (t:=t) f g.
+    Proof.
+      unfold interp_type_rel_pointwise2_uncurried_proj_option.
+      induction t as [t|A B IHt]; simpl; unfold Morphisms.respectful_hetero in *.
+      { induction t as [t|A IHA B IHB]; simpl; [ solve [ trivial | reflexivity ] | ].
+        intros [HA HB].
+        specialize (IHA _ _ HA); specialize (IHB _ _ HB).
+        unfold R in *.
+        repeat first [ progress destruct_head_hnf' prod
+                     | progress simpl in *
+                     | progress unfold LiftOption.of' in *
+                     | progress break_match
+                     | progress break_match_hyps
+                     | progress inversion_prod
+                     | progress inversion_option
+                     | reflexivity
+                     | progress intuition subst ]. }
+      { destruct B; intros H ?; apply IHt, H; clear IHt.
+        { repeat first [ progress simpl in *
+                       | progress unfold R, LiftOption.of' in *
+                       | progress break_match
+                       | reflexivity ]. }
+        { simpl in *; break_match; reflexivity. } }
+    Qed.
+  End proj_option.
+
+  Section proj_option2.
+    Context {interp_base_type1 : Type} {interp_base_type2 : Type}
+            (proj : interp_base_type1 -> interp_base_type2).
+
+    Let R {t : flat_type base_type} f g :=
+      let f' := LiftOption.of' (t:=t) f in
+      let g' := LiftOption.of' (t:=t) g in
+      match f', g' with
+      | Some f', Some g' => SmartVarfMap (fun _ => proj) f' = g'
+      | None, None => True
+      | Some _, _ => False
+      | None, _ => False
+      end.
+
+    Definition interp_type_rel_pointwise2_uncurried_proj_option2
+               {t : type base_type}
+      : interp_type (LiftOption.interp_base_type' interp_base_type1) t -> interp_type (LiftOption.interp_base_type' interp_base_type2) t -> Prop
+      := match t return interp_type (LiftOption.interp_base_type' interp_base_type1) t -> interp_type (LiftOption.interp_base_type' interp_base_type2) t -> Prop  with
+         | Tflat T => @R _
+         | Arrow A B
+           => fun f g
+              => forall x : interp_flat_type (fun _ => interp_base_type1) (all_binders_for (Arrow A B)),
+                  let y := SmartVarfMap (fun _ => proj) x in
+                  let fx := ApplyInterpedAll f (LiftOption.to' (Some x)) in
+                  let gy := ApplyInterpedAll g (LiftOption.to' (Some y)) in
+                  @R _ fx gy
+         end.
+
+    Lemma uncurry_interp_type_rel_pointwise2_proj_option2
+          {t : type base_type}
+          {f : interp_type (LiftOption.interp_base_type' interp_base_type1) t}
+          {g : interp_type (LiftOption.interp_base_type' interp_base_type2) t}
+      : interp_type_rel_pointwise2 (t:=t) (fun t => @R _) f g
+        -> interp_type_rel_pointwise2_uncurried_proj_option2 (t:=t) f g.
+    Proof.
+      unfold interp_type_rel_pointwise2_uncurried_proj_option2.
+      induction t as [t|A B IHt]; simpl; unfold Morphisms.respectful_hetero in *.
+      { induction t as [t|A IHA B IHB]; simpl; [ solve [ trivial | reflexivity ] | ].
+        intros [HA HB].
+        specialize (IHA _ _ HA); specialize (IHB _ _ HB).
+        unfold R in *.
+        repeat first [ progress destruct_head_hnf' prod
+                     | progress simpl in *
+                     | progress unfold LiftOption.of' in *
+                     | progress break_match
+                     | progress break_match_hyps
+                     | progress inversion_prod
+                     | progress inversion_option
+                     | reflexivity
+                     | progress intuition subst ]. }
+      { destruct B; intros H ?; apply IHt, H; clear IHt.
+        { repeat first [ progress simpl in *
+                       | progress unfold R, LiftOption.of' in *
+                       | progress break_match
+                       | reflexivity ]. }
+        { simpl in *; break_match; reflexivity. } }
+    Qed.
+  End proj_option2.
+
+  Section proj_from_option2.
+    Context {interp_base_type0 : Type} {interp_base_type1 interp_base_type2 : base_type -> Type}
+            (proj01 : forall t, interp_base_type0 -> interp_base_type1 t)
+            (proj02 : forall t, interp_base_type0 -> interp_base_type2 t)
+            (proj : forall t, interp_base_type1 t -> interp_base_type2 t).
+
+    Let R {t : flat_type base_type} f g :=
+      proj_eq_rel (SmartVarfMap proj (t:=t)) f g.
+
+    Definition interp_type_rel_pointwise2_uncurried_proj_from_option2
+               {t : type base_type}
+      : interp_type (LiftOption.interp_base_type' interp_base_type0) t -> interp_type interp_base_type1 t -> interp_type interp_base_type2 t -> Prop
+      := match t return interp_type _ t -> interp_type _ t -> interp_type _ t -> Prop  with
+         | Tflat T => fun f0 f g => match LiftOption.of' f0 with
+                                    | Some _ => True
+                                    | None => False
+                                    end -> @R _ f g
+         | Arrow A B
+           => fun f0 f g
+              => forall x : interp_flat_type (fun _ => interp_base_type0) (all_binders_for (Arrow A B)),
+                  let x' := SmartVarfMap proj01 x in
+                  let y' := SmartVarfMap proj x' in
+                  let fx := ApplyInterpedAll f x' in
+                  let gy := ApplyInterpedAll g y' in
+                  let f0x := LiftOption.of' (ApplyInterpedAll f0 (LiftOption.to' (Some x))) in
+                  match f0x with
+                  | Some _ => True
+                  | None => False
+                  end
+                  -> @R _ fx gy
+         end.
+
+    Lemma uncurry_interp_type_rel_pointwise2_proj_from_option2
+          {t : type base_type}
+          {f0}
+          {f : interp_type interp_base_type1 t}
+          {g : interp_type interp_base_type2 t}
+          (proj012 : forall t x, proj t (proj01 t x) = proj02 t x)
+      : interp_type_rel_pointwise2 (t:=t) (LiftOption.lift_relation (fun t => proj_eq_rel (proj01 t))) f0 f
+        -> interp_type_rel_pointwise2 (t:=t) (LiftOption.lift_relation (fun t => proj_eq_rel (proj02 t))) f0 g
+        -> interp_type_rel_pointwise2_uncurried_proj_from_option2 (t:=t) f0 f g.
+    Proof.
+      unfold interp_type_rel_pointwise2_uncurried_proj_from_option2.
+      induction t as [t|A B IHt]; simpl; unfold Morphisms.respectful_hetero in *.
+      { induction t as [t|A IHA B IHB]; simpl.
+        { cbv [LiftOption.lift_relation proj_eq_rel R].
+          break_match; try tauto; intros; subst.
+          apply proj012. }
+        { intros [HA HB] [HA' HB'] Hrel.
+          specialize (IHA _ _ _ HA HA'); specialize (IHB _ _ _ HB HB').
+          unfold R, proj_eq_rel in *.
+          repeat first [ progress destruct_head_hnf' prod
+                       | progress simpl in *
+                       | progress unfold LiftOption.of' in *
+                       | progress break_match
+                       | progress break_match_hyps
+                       | progress inversion_prod
+                       | progress inversion_option
+                       | reflexivity
+                       | progress intuition subst ]. } }
+      { destruct B; intros H0 H1 ?; apply IHt; clear IHt; first [ apply H0 | apply H1 ];
+          repeat first [ progress simpl in *
+                       | progress unfold R, LiftOption.of', proj_eq_rel, LiftOption.lift_relation in *
+                       | break_match; rewrite <- ?proj012; reflexivity ]. }
+    Qed.
+  End proj_from_option2.
+  Global Arguments uncurry_interp_type_rel_pointwise2_proj_from_option2 {_ _ _ _ _} proj {t f0 f g} _ _ _.
+
+  Section proj1_from_option2.
+    Context {interp_base_type0 interp_base_type1 : Type} {interp_base_type2 : base_type -> Type}
+            (proj01 : interp_base_type0 -> interp_base_type1)
+            (proj02 : forall t, interp_base_type0 -> interp_base_type2 t)
+            (R : forall t, interp_base_type1 -> interp_base_type2 t -> Prop).
+
+    Definition interp_type_rel_pointwise2_uncurried_proj1_from_option2
+               {t : type base_type}
+      : interp_type (LiftOption.interp_base_type' interp_base_type0) t -> interp_type (LiftOption.interp_base_type' interp_base_type1) t -> interp_type interp_base_type2 t -> Prop
+      := match t return interp_type _ t -> interp_type _ t -> interp_type _ t -> Prop  with
+         | Tflat T => fun f0 f g => match LiftOption.of' f0 with
+                                    | Some _ => True
+                                    | None => False
+                                    end -> match LiftOption.of' f with
+                                           | Some f' => interp_flat_type_rel_pointwise2 (@R) f' g
+                                           | None => True
+                                           end
+         | Arrow A B
+           => fun f0 f g
+              => forall x : interp_flat_type (fun _ => interp_base_type0) (all_binders_for (Arrow A B)),
+                  let x' := SmartVarfMap (fun _ => proj01) x in
+                  let y' := SmartVarfMap proj02 x in
+                  let fx := LiftOption.of' (ApplyInterpedAll f (LiftOption.to' (Some x'))) in
+                  let gy := ApplyInterpedAll g y' in
+                  let f0x := LiftOption.of' (ApplyInterpedAll f0 (LiftOption.to' (Some x))) in
+                  match f0x with
+                  | Some _ => True
+                  | None => False
+                  end
+                  -> match fx with
+                     | Some fx' => interp_flat_type_rel_pointwise2 (@R) fx' gy
+                     | None => True
+                     end
+         end.
+
+    Lemma uncurry_interp_type_rel_pointwise2_proj1_from_option2
+          {t : type base_type}
+          {f0}
+          {f : interp_type (LiftOption.interp_base_type' interp_base_type1) t}
+          {g : interp_type interp_base_type2 t}
+          (proj012R : forall t x, @R _ (proj01 x) (proj02 t x))
+      : interp_type_rel_pointwise2 (t:=t) (LiftOption.lift_relation2 (proj_eq_rel proj01)) f0 f
+        -> interp_type_rel_pointwise2 (t:=t) (LiftOption.lift_relation (fun t => proj_eq_rel (proj02 t))) f0 g
+        -> interp_type_rel_pointwise2_uncurried_proj1_from_option2 (t:=t) f0 f g.
+    Proof.
+      unfold interp_type_rel_pointwise2_uncurried_proj1_from_option2.
+      induction t as [t|A B IHt]; simpl; unfold Morphisms.respectful_hetero in *.
+      { induction t as [t|A IHA B IHB]; simpl.
+        { cbv [LiftOption.lift_relation proj_eq_rel LiftOption.lift_relation2].
+          break_match; try tauto; intros; subst.
+          apply proj012R. }
+        { intros [HA HB] [HA' HB'] Hrel.
+          specialize (IHA _ _ _ HA HA'); specialize (IHB _ _ _ HB HB').
+          unfold proj_eq_rel in *.
+          repeat first [ progress destruct_head_hnf' prod
+                       | progress simpl in *
+                       | progress unfold LiftOption.of' in *
+                       | progress break_match
+                       | progress break_match_hyps
+                       | progress inversion_prod
+                       | progress inversion_option
+                       | reflexivity
+                       | progress intuition subst ]. } }
+      { destruct B; intros H0 H1 ?; apply IHt; clear IHt; first [ apply H0 | apply H1 ];
+          repeat first [ progress simpl in *
+                       | progress unfold R, LiftOption.of', proj_eq_rel, LiftOption.lift_relation in *
+                       | break_match; reflexivity ]. }
+    Qed.
+  End proj1_from_option2.
+  Global Arguments uncurry_interp_type_rel_pointwise2_proj1_from_option2 {_ _ _ _ _} R {t f0 f g} _ _ _.
+
+  Section combine_related.
+    Lemma related_flat_transitivity {interp_base_type1 interp_base_type2 interp_base_type3}
+          {R1 : forall t : base_type, interp_base_type1 t -> interp_base_type2 t -> Prop}
+          {R2 : forall t : base_type, interp_base_type1 t -> interp_base_type3 t -> Prop}
+          {R3 : forall t : base_type, interp_base_type2 t -> interp_base_type3 t -> Prop}
+          {t x y z}
+    : (forall t a b c, (R1 t a b : Prop) -> (R2 t a c : Prop) -> (R3 t b c : Prop))
+      -> interp_flat_type_rel_pointwise2 (t:=t) R1 x y
+      -> interp_flat_type_rel_pointwise2 (t:=t) R2 x z
+      -> interp_flat_type_rel_pointwise2 (t:=t) R3 y z.
+    Proof.
+      intro HRel; induction t; simpl; intuition eauto.
+    Qed.
+  End combine_related.
+End Relations.
