src/Specific/GF25519Reflective/CommonUnOp.v
@@ -1,6 +1,6 @@
 Require Export Crypto.Specific.GF25519Reflective.Common.
 Require Import Crypto.Specific.GF25519BoundedCommon.
-Require Import Crypto.Reflection.Z.Interpretations.
+Require Import Crypto.Reflection.Z.Interpretations64.
 Require Import Crypto.Reflection.Syntax.
 Require Import Crypto.Reflection.Application.
 Require Import Crypto.Reflection.MapInterp.
@@ -15,7 +15,7 @@ Lemma ExprUnOp_correct_and_bounded
                    (Hx : is_bounded (fe25519WToZ x) = true),
           let args := unop_args_to_bounded x Hx in
           match LiftOption.of'
-                  (ApplyInterpedAll (Interp (@BoundedWord64.interp_op) (MapInterp BoundedWord64.of_word64 ropW))
+                  (ApplyInterpedAll (Interp (@BoundedWordW.interp_op) (MapInterp BoundedWordW.of_wordW ropW))
                                     (LiftOption.to' (Some args)))
           with
           | Some _ => True
@@ -25,9 +25,9 @@ Lemma ExprUnOp_correct_and_bounded
                    (x := eta_fe25519W x)
                    (Hx : is_bounded (fe25519WToZ x) = true),
           let args := unop_args_to_bounded x Hx in
-          let x' := SmartVarfMap (fun _ : base_type => BoundedWord64.BoundedWordToBounds) args in
+          let x' := SmartVarfMap (fun _ : base_type => BoundedWordW.BoundedWordToBounds) args in
           match LiftOption.of'
-                  (ApplyInterpedAll (Interp (@ZBounds.interp_op) (MapInterp ZBounds.of_word64 ropW)) (LiftOption.to' (Some x')))
+                  (ApplyInterpedAll (Interp (@ZBounds.interp_op) (MapInterp ZBounds.of_wordW ropW)) (LiftOption.to' (Some x')))
           with
           | Some bounds => unop_bounds_good bounds = true
           | None => False
